\begin{itemize}

\item algorithm

\item Theoretical models and technicalities

\end{itemize}

\subsection{Algorithm}

\subsection{The general tridiagonal matrix}
The algorithm is first written for an equation with a general tridiagonal matrix on the short form:
\[
\mathbf{A}\mathbf{v}=\mathbf{b}
\]
The full form looks like this:
\[
    \begin{bmatrix}
    	d_1& e_1& 0 &\cdots & 0 &0 \\
        c_1 & d_2 & e_2 &0 &\cdots &0 \\
        0&c_2 &d_3 & e_3 & \cdots & 0 \\
        \vdots& \vdots & \ddots &\ddots &\ddots & \vdots \\
        0&0 & \cdots &c_{n-2} &d_{n-1}& e_{n-1} \\
        0&0 & \cdots & 0  &c_{n-1} & d_n \\
        \end{bmatrix}
\begin{bmatrix}
	v_1\\
	v_2\\
	v_3\\
	\vdots\\
	v_{n-1}\\
	v_{n}\\
\end{bmatrix}=
\begin{bmatrix}
	b_1\\
	b_2\\
	b_3\\
	\vdots\\
	b_{n-1}\\
	b_{n}\\
\end{bmatrix}
\]

The method used to solve the equation numerically was to first to a forward substitution to obtain a upper triangular matrix and then a backwards substitution to obtain the solution.

The algorithm preformed on the matrix values was:

\paragraph{The forward substitution:\hspace{4cm}}

\hspace{1cm}\linebreak
The values on the diagonal:
\[
\tilde{d_i} =  d_i - \left(\frac{c_i \cdot e_i}{\tilde{d}_{i-1}}\right)\linebreak
\]
The values on the right side of the equation:
\[
\tilde{b_i} =  b_i - \left(\frac{\tilde{b}_{i-1} \cdot e_i}{\tilde{d}_{i-1}}\right)
\]
for $i = 2, \dots, n-2 $

\paragraph{The backwards substitution:\hspace{4cm}}

\hspace{1cm}\linebreak
\[
v_i = \frac{\left(\tilde{b}_i + v_{i+1}\right)}{\tilde{d}_i}
\]
for $i = 2, \dots, n-2 $. The boundary values are known ($v_0 = v_n = 0$). $v_{n-1}$ was calculated first and like this:
\[
v_{n-1} = \frac{\tilde{b}_{n-1}}{\tilde{d}_{n-1}}
\]

\subsection{This specific tridiagonal matrix}

The matrix in our case had the same values on the different diagonals:
\begin{multicols}{3}
\[
d_i = 2
\]

\[
e_i = -1
\]

\[
c_i = -1
\]
\end{multicols}

We can then pre-calculate some of the operations in the algorithm and if becomes then:

\paragraph{The forward substitution:\hspace{4cm}}

\hspace{1cm}\linebreak
The values on the diagonal:
\[
\tilde{d_i} =  d_i - \left(\frac{c_i \cdot e_i}{\tilde{d}_{i-1}}\right) = 2 - \left(\frac{(-1) \cdot (-1)}{\tilde{d}_{i-1}}\right) = \frac{i + 1}{i}
\]
The values on the right side of the equation:
\[
\tilde{b_i} =  b_i - \left(\frac{\tilde{b}_{i-1} \cdot e_i}{\tilde{d}_{i-1}}\right) = b_i - \left(\frac{\tilde{b}_{i-1} \cdot (-1)}{\tilde{d}_{i-1}}\right) = b_i + \left(\frac{\tilde{b}_{i-1}}{\tilde{d}_{i-1}}\right)
\]
for $i = 2,\, \dots\, , n-2 $.

\paragraph{The backwards substitution:\hspace{4cm}}

\hspace{1cm}\linebreak
\[
v_i = \frac{\left(\tilde{b}_i + v_{i+1}\right)}{\tilde{d}_i}
\]
for $i = 2, \dots, n-2 $. The boundary values are known ($v_0 = v_n = 0$). $v_{n-1}$ was calculated first and like this:
\[
v_{n-1} = \frac{\tilde{b}_{n-1}}{\tilde{d}_{n-1}}
\]

\subsection{LU-composition}